(a)
\textsc{Answer:}\vspace{-2mm}
\begin{answerlong}
\begin{align*}
110010_2 &= 1 \cdot 2^{5} + 1\cdot 2^{4} + 0 \cdot 2^{3} + 0\cdot 2^{2} + 1\cdot 2^{1} + 0\cdot 2^{0} \\
         &= 32 + 16 + 0 + 0 + 2 + 0 \\
         &= 50
\end{align*}
Therefore $110010_{2} = 50$.
\end{answerlong}

(b)
\textsc{Answer:}\vspace{-2mm}
\begin{answerlong}
\begin{align*}
110010_2 &= 1 \cdot 2^{5} + 1\cdot 2^{4} + 0 \cdot 2^{3} + 0\cdot 2^{2} + 1 \cdot 2^{1} + 0\cdot 2^{0} \\
         &= (1 \cdot 2^{1} + 1\cdot 2^{0})2^{4} + (0 \cdot 2^{1} + 0\cdot 2^{0})2^{2} +(1 \cdot 2^{1} + 0\cdot 2^{0}) 2^{0} \\
         &= (1 \cdot 2^{1} + 1\cdot 2^{0})(2^{2})^{2} + (0 \cdot 2^{1} + 0\cdot 2^{0})(2^{2})^{1} +(1 \cdot 2^{1} + 0\cdot 2^{0})(2^{2})^{0}  \\
         &= (1 \cdot 2^{1} + 1\cdot 2^{0})4^{2} + (0 \cdot 2^{1} + 0\cdot 2^{0})4^{1} +(1 \cdot 2^{1} + 0\cdot 2^{0})4^{0} \\
         &= (3)4^{2} + (0)4^{1} + (2)4^{0} \\
         &= 302_{4}
\end{align*}
Therefore $110010_{2} = 302_{4}$.
\end{answerlong}

(c)
\textsc{Answer:}\vspace{-2mm}
\begin{answerlong}
\begin{align*}
110010_2 &= 1 \cdot 2^{5} + 1\cdot 2^{4} + 0 \cdot 2^{3} + 0\cdot 2^{2} + 1 \cdot 2^{1} + 0\cdot 2^{0} \\
         &= (1 \cdot 2^{2} + 1\cdot 2^{1} + 0 \cdot 2^{0})2^{3} + (0\cdot 2^{2} + 1 \cdot 2^{1} + 0\cdot 2^{0})2^{0} \\
         &= (1 \cdot 2^{2} + 1\cdot 2^{1} + 0 \cdot 2^{0})(2^{3})^{1} + (0\cdot 2^{2} + 1 \cdot 2^{1} + 0\cdot 2^{0})(2^{3})^{0} \\
         &= (1 \cdot 2^{2} + 1\cdot 2^{1} + 0 \cdot 2^{0})8^{1} + (0\cdot 2^{2} + 1 \cdot 2^{1} + 0\cdot 2^{0})8^{0} \\
         &= (4 + 2 + 0)8^{1} + (0 + 2 + 0)8^{0} \\
         &= (6)8^{1} + (2)8^{0}\\
         &= 62_{8}
\end{align*}
Therefore $110010_2 = 62_{8}$.
\end{answerlong}

(d)
\textsc{Answer:}\vspace{-2mm}
\begin{answerlong}
\begin{align*}
110010_2 &= 1 \cdot 2^{5} + 1\cdot 2^{4} + 0 \cdot 2^{3} + 0\cdot 2^{2} + 1 \cdot 2^{1} + 0\cdot 2^{0} \\
         &= (1 \cdot 2^{1} + 1\cdot 2^{0})2^{4} + (0 \cdot 2^{3} + 0\cdot 2^{2} + 1 \cdot 2^{1} + 0\cdot 2^{0})2^{0} \\
         &= (1 \cdot 2^{1} + 1\cdot 2^{0})(2^{4})^{1} + (0 \cdot 2^{3} + 0\cdot 2^{2} + 1 \cdot 2^{1} + 0\cdot 2^{0})(2^{4})^{0} \\
         &= (1 \cdot 2^{1} + 1\cdot 2^{0})16^{1} + (0 \cdot 2^{3} + 0\cdot 2^{2} + 1 \cdot 2^{1} + 0\cdot 2^{0})16^{0} \\
         &= (2 + 1)16^{1} + (0 + 0 + 2 + 0)16^{0} \\
         &= (3)16^{1} + (2)16^{0} \\
         &= 32_{16}
\end{align*}
Therefore $110010_2 = 32_{16}$.
\end{answerlong}
